src/Utils.ec
@@ -7,6 +7,8 @@ require import Logic.
 require import UInt256.
 import StdOrder.
 
+prover timeout=20.
+
   (* option *)
 
 lemma exists_of_is_some ['a] (ov : 'a option) : is_some ov => exists (v : 'a), ov = Some v. progress. smt (). qed.
@@ -53,6 +55,14 @@ lemma mul_add_mod_eq (a b m : int) : 0 < m => ((m * a) + b) %% m = b %% m.
   qed.
 
 lemma add_mod_mod_eq_add_mod (a b m : int) : (a + (b %% m)) %% m = (a + b) %% m.
+    smt (@IntDiv).
+  qed.
+
+ lemma add_mod_eq_mod_add_mod_mod (a b m : int) : (a + b) %% m = ((a %% m) + (b %% m)) %% m.
+    smt (@IntDiv).
+  qed.
+
+lemma mul_mod_eq_mod_mul_mod_mod (a b m : int) : (a * b) %% m = ((a %% m) * (b %% m)) %% m.
     smt (@IntDiv).
   qed.
   
